Prove frame rule at single perm level, but doesn't work for perm sets

src/Yield.v
@@ -37,95 +37,130 @@ Ltac rewritebisim_in lem H := pose proof lem as bisim;
 Variant yieldE S : Type -> Type :=
 | Yield : S -> yieldE S S.
 
+(** return one of the elements in [x :: xs], as well as the complete list of unchosen elements *)
+Fixpoint choose' {E} `{nondetE -< E} {X} (x : X) (xs : list X) (rest : list X) :
+  itree E (X * list X)
+  := match xs with
+     | [] => Ret (x, rest)
+     | x' :: xs => or
+                   (Ret (x, (x' :: xs) ++ rest)) (* [x] *)
+                   (choose' x' xs (x :: rest)) (* not [x] *)
+     end.
+Definition choose {E} `{nondetE -< E} {X} x xs : itree E (X * list X) :=
+  choose' x xs [].
+
+Definition E config := yieldE config +' nondetE.
+
 Section parallel.
   Parameter config : Type.
 
-  Definition thread := stateT config (itree (yieldE config)) unit.
+  Definition thread := stateT config (itree (E config)) unit.
 
-  Definition choose {E} `{nondetE -< E} {X}
-    : X -> list X -> list X -> itree E (X * list X)
-    := fix choose1' x xs rest : itree E (X * list X) :=
-         match xs with
-         | [] => Ret (x, rest)
-         | x' :: xs => or (Ret (x, (x' :: xs) ++ rest)) (choose1' x' xs (x :: rest))
-         end.
-
+  (** Interprets away yields *)
   Definition par_match par (curr : thread) (rest : list thread)
-    : stateT config (itree nondetE) unit :=
+    : thread :=
     fun s =>
       match (observe (curr s)) with
       | RetF (s', _) => match rest with
-                       | nil => Ret (s', tt)
-                       | cons h t => Tau (par h t s')
+                       | [] => Ret (s', tt)
+                       | h :: t => Tau (par h t s')
                        end
       | TauF t => Tau (par (fun _ => t) rest s)
-      | VisF (Yield _ s') k =>
-        '(curr', rest') <- choose k rest [];;
-        Tau (par curr' rest' s')
+      | VisF (inl1 e) k =>
+        match e in yieldE _ C return (C -> itree (E config) (config * unit)) -> _ with
+        | Yield _ s' =>
+          fun k' =>
+          '(curr', rest') <- choose k' rest;;
+          Tau (par curr' rest' s')
+        end k
+      | VisF (inr1 e) k =>
+        vis e (fun b => par (fun _ => k b) rest s)
       end.
   CoFixpoint par := par_match par.
   Lemma rewrite_par curr rest : par curr rest = par_match par curr rest.
   Proof.
-  Admitted.
+    apply functional_extensionality. intros. apply bisimulation_is_eq.
+    revert x curr rest.
+    ginit. gcofix CIH. intros. gstep. unfold par. red. reflexivity.
+  Qed.
 
+  Lemma par_single :
+    forall t, par t [] = t.
+  Proof.
+    intro. apply functional_extensionality. intros. apply bisimulation_is_eq.
+    revert t x. pcofix CIH. intros.
+    rewrite rewrite_par. unfold par_match.
+    destruct (observe (t x)) eqn:?; simpl; auto.
+    - destruct r0. pstep. red. rewrite Heqi. simpl. destruct u. constructor; auto.
+    - pstep. red. rewrite Heqi. constructor. right. apply CIH.
+    - destruct e.
+      + destruct y. pstep. unfold choose. unfold choose'.
+        rewritebisim @bind_ret_l.
+  Abort.
+
+  (* Not true using ≅, need equivalence that involves nondeterminism: *)
   (* Lemma par_unit : *)
-  (*   forall t, par (fun s => Ret (s, tt)) [t] = par t [fun s => Ret (s, tt)]. *)
+  (*   forall t s, par (fun s => Ret (s, tt)) [t] s ≅ par t [fun s => Ret (s, tt)] s. *)
   (* Proof. *)
-  (*   intros. do 2 rewrite rewrite_par. *)
-  (*   unfold par_match. apply functional_extensionality. intros. simpl. *)
-  (*   destruct (observe (t x)) eqn:?. *)
-  (*   - destruct r. admit. *)
-  (*   - admit. *)
+  (*   intros. rewrite rewrite_par. unfold par_match. simpl. *)
+  (*   (* do 2 rewrite rewrite_par. *) *)
+  (*   rewrite (rewrite_par t [_]). *)
+  (*   unfold par_match. simpl. *)
+  (*   destruct (observe (t s)) eqn:?. *)
+  (*   - destruct r. pstep. (* rewrite rewrite_par. unfold par_match. *) constructor. *)
+  (*     left. *)
+  (*     do 2 rewrite rewrite_par. unfold par_match. rewrite Heqi. simpl. *)
+  (*     pstep. constructor; auto. *)
+  (*   - pstep. constructor. left. revert Heqi. revert t t0 s. pcofix CIH. intros. *)
+  (*     do 2 rewrite rewrite_par. unfold par_match. rewrite Heqi. *)
+  (*     rewrite (rewrite_par (fun _ => t0) _). unfold par_match. rewrite Heqi. simpl. *)
   (*   - destruct e. *)
   (* Qed. *)
 End parallel.
 
-Definition E config := yieldE config +' nondetE.
-
-Variant typing_gen {config R} typing (p : perm) (Q : R -> Perms) :
+Variant typing_gen {R} typing (p : perm) (Q : config * R -> Perms) :
   config -> itree (E config) (config * R) -> Prop :=
-  (* stateT config (itree (yieldE config)) R -> Prop := *)
 | typing_gen_ret r c c' :
     pre p c ->
-    p ∈ Q r ->
+    p ∈ Q (c', r) ->
     guar p c c' ->
     typing_gen typing p Q c (Ret (c', r))
-| typing_gen_tau t c :
+| typing_gen_tau t c p' :
     pre p c ->
-    typing p Q c t ->
+    sep_step p p' -> (* Added since par turns vis into a tau, so the two cases need to be similar... *)
+    typing p' Q c t ->
     typing_gen typing p Q c (Tau t)
 | typing_gen_vis k c c' p' :
     pre p c ->
     guar p c c' ->
     sep_step p p' ->
-    (forall c'', rely p c' c'' -> typing p' Q c'' (k c'')) ->
+    (forall c'', rely p c' c'' -> typing p' Q c (* c'? *) (k c'')) ->
     typing_gen typing p Q c (vis (Yield _ c') k).
 
-Lemma typing_gen_mon {config R} : monotone4 (@typing_gen config R).
+Lemma typing_gen_mon {R} : monotone4 (@typing_gen R).
 Proof.
   repeat intro. inversion IN; subst; econstructor; eauto.
 Qed.
 Hint Resolve typing_gen_mon : paco.
 
-Definition typing_ {config R} := paco4 (@typing_gen config R) bot4.
+Definition typing_ {R} := paco4 (@typing_gen R) bot4.
 
-Lemma typing__lte {config R} p (Q Q' : R -> Perms) (c : config) t :
+Lemma typing__lte {R} p Q Q' c (t : itree (E config) (config * R)) :
   typing_ p Q c t ->
   (forall r, Q r ⊨ Q' r) ->
   typing_ p Q' c t.
 Proof.
   revert p Q Q' c t. pcofix CIH. intros p Q Q' c t Htyping Hlte.
-  punfold Htyping. pstep.
-  inversion Htyping; pclearbot; subst; econstructor; eauto.
+  pstep. pinversion Htyping; pclearbot; subst; econstructor; eauto.
   - apply Hlte; eauto.
-  - intros. specialize (H2 _ H3). pclearbot. right. eapply CIH; eauto.
+  - intros. specialize (H2 _ H3). pclearbot. eauto.
 Qed.
 
-Definition typing {config R} P Q (t : stateT config (itree (E config)) R) :=
+Definition typing {R} P Q (t : stateT config (itree (E config)) R) :=
   forall p c c', p ∈ P -> pre p c -> guar p c c' -> typing_ p Q c (t c').
 (* also pre p c'? *)
 
-Lemma typing_lte {config R} P P' Q Q' (t : stateT config (itree (E config)) R) :
+Lemma typing_lte {R} P P' Q Q' (t : stateT config (itree (E config)) R) :
   typing P Q t ->
   P' ⊨ P ->
   (forall r, Q r ⊨ Q' r) ->
@@ -134,29 +169,162 @@ Proof.
   repeat intro. eapply typing__lte; eauto.
 Qed.
 
-Lemma typing__bind {config R S} p (Q1 : R -> Perms) (Q2 : S -> Perms) (c : config) t1 t2 r' :
-  pre p c ->
+Lemma typing__bind {R S} p Q1 Q2 c
+      (t1 : itree (E config) (config * R))
+      (t2 : R -> stateT config (itree (E config)) S)
+      r' :
   typing_ p Q1 c t1 ->
-  (forall r p c c', p ∈ Q1 r ->
+  (forall r p c c', p ∈ Q1 (c', r) ->
                pre p c ->
                guar p c c' ->
                paco4 typing_gen r' p Q2 c (t2 r c')) ->
   paco4 typing_gen r' p Q2 c (x <- t1;; t2 (snd x) (fst x)).
 Proof.
-  revert p Q1 Q2 c t1 t2. pcofix CIH. intros p Q1 Q2 c t1 t2 Hpre Htyping1 Htyping2.
+  revert p Q1 Q2 c t1 t2. pcofix CIH. intros p Q1 Q2 c t1 t2 Htyping1 Htyping2.
   pinversion Htyping1; subst.
   - rewritebisim @bind_ret_l. eapply paco4_mon; eauto.
   - rewritebisim @bind_tau. pstep. econstructor; eauto.
   - rewritebisim @bind_vis. pstep. econstructor; eauto. intros.
     specialize (H2 _ H3). pclearbot. right. eapply CIH; eauto.
-    pinversion H2; auto.
 Qed.
 
-Lemma typing_bind {config R S} P Q1 Q2 (t1 : stateT config (itree (E config)) R) (t2 : R -> stateT config (itree (E config)) S) :
+Lemma typing_bind {R S} P Q1 Q2
+      (t1 : stateT config (itree (E config)) R)
+      (t2 : R -> stateT config (itree (E config)) S) :
   typing P Q1 t1 ->
-  (forall r, typing (Q1 r) Q2 (t2 r)) ->
+  (forall c r, typing (Q1 (c, r)) Q2 (t2 r)) ->
   typing P Q2 (bind t1 t2).
 Proof.
   repeat intro. unfold bind. unfold Monad_stateT. red.
-  eapply typing__bind; eauto.
+  eapply typing__bind; eauto. intros. eapply H0; eauto.
+Qed.
+
+Lemma typing__sep_step p p' Q c (t : itree (E config) (config * unit)) :
+  sep_step p p' ->
+  typing_ p' Q c t ->
+  typing_ p Q c t.
+Proof.
+  revert c t. pcofix CIH. intros c t Hstep Ht.
+  punfold Ht. induction Ht.
+  - pstep. constructor; auto.
+Abort.
+
+Lemma typing__par_empty p Q c c' t :
+  typing_ p Q c (t c') ->
+  typing_ p Q c (par t [] c').
+Proof.
+  revert p c c' t.
+  pcofix CIH.
+  intros p c c' t Ht. rewrite rewrite_par. unfold par_match.
+  pinversion Ht; subst; simpl.
+  - pstep. constructor; auto. destruct r0; auto.
+  - pstep. econstructor; eauto.
+  - pstep. unfold choose, choose'. rewritebisim @bind_ret_l. econstructor; eauto.
+    right. eapply CIH; eauto.
+    assert (rely p c'0 c'0) by reflexivity.
+    specialize (H4 _ H3). pclearbot. eauto.
+Qed.
+
+Lemma typing_par_empty P Q t :
+  typing P Q t ->
+  typing P Q (par t []).
+Proof.
+  intros Ht p c c' Hp Hpre Hguar. apply typing__par_empty; auto.
+Qed.
+
+(* Lemma typing__par_empty' p Q Q' c c' t : *)
+(*   p ∈ Q' tt -> *)
+(*   typing_ p Q c (t c') -> *)
+(*   typing_ p Q c (par t [] c'). *)
+(* Proof. *)
+(*   revert p c c' t. *)
+(*   pcofix CIH. *)
+(*   intros p c c' t Ht. rewrite rewrite_par. unfold par_match. *)
+(*   pinversion Ht; subst; simpl. *)
+(*   - pstep. constructor; auto. destruct r0; auto. *)
+(*   - pstep. econstructor; eauto. *)
+(*   - pstep. unfold choose, choose'. rewritebisim @bind_ret_l. econstructor; eauto. *)
+(*     right. eapply CIH; eauto. *)
+(*     assert (rely p c'0 c'0) by reflexivity. *)
+(*     specialize (H4 _ H3). pclearbot. eauto. *)
+(* Qed. *)
+
+Lemma typing__frame p p' r (Q : config * unit -> Perms) R t c :
+  typing_ p Q c t ->
+  r ∈ R ->
+  p ** r <= p' ->
+  pre p' c ->
+  typing_ p' (fun c => Q c * R) c t.
+Proof.
+  revert p p' r Q R t c.
+  pcofix CIH. intros p p' r' Q R t c Ht Hr Hp' Hpre.
+  pinversion Ht; subst.
+  - pstep. constructor; auto.
+    + eapply Perms_upwards_closed; eauto. apply sep_conj_Perms_perm; auto.
+    + apply Hp'. constructor. left. auto.
+  - pstep. econstructor; auto.
+    + eapply sep_step_lte; eauto. eapply sep_step_sep_conj_l.
+      apply Hp' in Hpre. apply Hpre.
+      apply H0.
+    + right. eapply CIH; eauto. reflexivity.
+      split; [| split]. pinversion H1; auto.
+      apply Hp'. apply Hpre.
+      apply H0. apply Hp' in Hpre. apply Hpre.
+  - pstep. econstructor; eauto.
+    + apply Hp'. constructor. left. auto.
+    + eapply sep_step_lte; eauto. eapply sep_step_sep_conj_l.
+      apply Hp' in Hpre. apply Hpre.
+      apply H1.
+    + intros. right.
+      assert (rely p c' c'').
+      { apply Hp'. auto. }
+      specialize (H2 _ H4). pclearbot.
+      eapply CIH; eauto. reflexivity.
+      split; [| split]. pinversion H2; auto.
+      apply Hp'. apply Hpre.
+      apply H1. apply Hp' in Hpre. apply Hpre.
+Qed.
+
+Lemma typing_frame P P' (Q : config * unit -> Perms) t :
+  typing P Q t ->
+  typing (P * P') (fun r => Q r * P') t.
+Proof.
+  repeat intro. destruct H0 as (? & ? & ? & ? & ?).
+  eapply typing__frame; eauto. apply H; auto. apply H4. auto. inversion H4.
+  (* intros Ht p c c' Hp Hpre Hguar. *)
+  revert P P' Q t. pcofix CIH. intros P P' Q t Ht p c c' Hp Hpre Hguar.
+  assert (Hp': p ∈ P).
+  { destruct Hp as (? & ? & ? & ? & ?).
+    eapply Perms_upwards_closed; eauto. etransitivity; eauto.
+    apply lte_l_sep_conj_perm. }
+  specialize (Ht _ _ _ Hp' Hpre Hguar).
+  (* revert Ht Hp Hpre Hguar Hp'. revert P P' Q t p c c'. pcofix CIH. *)
+  (* intros P P' Q t p c c' Ht Hpp' Hpre Hguar Hp. *)
+
+  pinversion Ht; subst.
+  - pstep. constructor; auto. admit.
+  - pstep. econstructor. auto. reflexivity. right.
+    change t0 with ((fun _ => t0) c'). eapply CIH; eauto.
+    repeat intro.
+
+Qed.
+
+Lemma typing_par P1 P2 (Q1 Q2 : config * unit -> Perms) t1 t2 :
+  typing P1 Q1 t1 ->
+  typing P2 Q2 t2 ->
+  typing (P1 * P2) (fun '(c, _) => Q1 (c, tt) * Q2 (c, tt)) (par t1 [t2]).
+Proof.
+  revert t1 t2 P1 P2 Q1 Q2.
+  pcofix CIH. intros t1 t2 P1 P2 Q1 Q2.
+  intros Ht1 Ht2 p c c' (p1 & p2 & Hp1 & Hp2 & Hlte) Hpre Hguar.
+  rewrite rewrite_par. unfold par_match.
+  assert (Hp1': p ∈ P1) by admit.
+  specialize (Ht1 _ _ _ Hp1' Hpre Hguar). pinversion Ht1; subst; simpl.
+  - destruct r0. pstep. econstructor; eauto. reflexivity. left.
+    (* How do we push through the stronger post-condition here? p can change arbitrarily in the typing computation for t2, so why does this hold? *)
+    eapply typing_par_empty in Ht2.
+    red in Ht2.
+    eapply paco4_mon_bot. apply Ht2; eauto. admit.
+    intros. eauto.
+  -
 Qed.
